progs/verif_sha_bdo3.v
@@ -90,12 +90,13 @@ reflexivity.
 Qed.
 
 Lemma rearrange_aux2: 
-forall (Espec : OracleKind) (i : nat)(w k : int)
-  (regs' : registers) (a b c d e f g h : int) (eqofs : val -> Prop),
+forall (Espec : OracleKind) (i : nat)(w k : int) ctx
+      (a b c d e f g h : int) (eqofs : val -> Prop),
 i < 16 ->
 semax (initialized _Ki (initialized _l (initialized _l' Delta_loop1)))
   (PROP  ()
-   LOCAL  (`eqofs (eval_id _data); `(eq (Vint w)) (eval_id _l);
+   LOCAL  (`(eq ctx) (eval_id _ctx);
+   `eqofs (eval_id _data); `(eq (Vint w)) (eval_id _l);
    `(eq (Vint k)) (eval_id _Ki);
    `(eq (Vint (Int.repr (Z.of_nat i)))) (eval_id _i);
    `(eq (map Vint [a, b, c, d, e, f, g, h]))
@@ -109,7 +110,8 @@ semax (initialized _Ki (initialized _l (initialized _l' Delta_loop1)))
    SEP()) rearrange_regs
   (normal_ret_assert
      (PROP  (S i <= 16)
-      LOCAL  (`(eq (Vint (Int.repr (Z.of_nat i)))) (eval_id _i);
+      LOCAL  (`(eq ctx) (eval_id _ctx);
+   `(eq (Vint (Int.repr (Z.of_nat i)))) (eval_id _i);
       `eqofs (eval_id _data);
       `(eq (map Vint (rnd_function [a, b, c, d, e, f, g, h]  k w)))
         (`cons (eval_id _a)
@@ -121,6 +123,7 @@ semax (initialized _Ki (initialized _l (initialized _l' Delta_loop1)))
                           (`cons (eval_id _g) (`cons (eval_id _h) `[])))))))))
         SEP())).
 Proof.
+(*
 {
 intros.
 name a_ _a.
@@ -137,6 +140,7 @@ name i_ _i.
 name T1 _T1.
 name T2 _T2.
 name data_ _data.
+name ctx_ _ctx.
 unfold Delta_loop1; simplify_Delta.
 simpl.
 unfold rearrange_regs.
@@ -152,7 +156,6 @@ repeat match goal with
  | H: _ = eval_id _ rho |- _ => rewrite <- H in *; clear H
 end.
 repeat split; auto.
-clear H13 H0 rho H1 H19 Delta.
 clear.
 cbv beta iota delta [sem_and sem_notint sem_or sem_shl sem_shr sem_or sem_add sem_xor]; simpl.
 repeat rewrite <- Sigma_1_eq.
@@ -162,17 +165,19 @@ repeat rewrite <- Maj_eq.
 repeat rewrite (rearrange_aux h).
 reflexivity.
 }
+*)
 Admitted.  (* can't Qed, because it goes over 2 gigabytes *)
 
 Lemma rearrange_regs_proof:
- forall (Espec: OracleKind) i (data: val) bl regs
+ forall (Espec: OracleKind) i (data: val) bl regs ctx
  (Hdata: isptr data)
  (H: length bl = LBLOCK)
  (H0: i < 16), 
  semax (initialized _Ki (initialized _l (initialized _l' Delta_loop1)))
   (PROP  ()
    LOCAL 
-   (`(eq (offset_val (Int.repr (Zsucc (Z.of_nat i) * 4)) data)) (eval_id _data);
+   (`(eq ctx) (eval_id _ctx);
+   `(eq (offset_val (Int.repr (Zsucc (Z.of_nat i) * 4)) data)) (eval_id _data);
    `(eq (Vint (big_endian_integer
              (fun z : Z =>
               force_option Int.zero
@@ -192,7 +197,8 @@ Lemma rearrange_regs_proof:
    SEP()) rearrange_regs
   (normal_ret_assert
      (PROP  (S i <= 16)
-      LOCAL  (`(eq (Vint (Int.repr (Z.succ (Z.of_nat i) - 1)))) (eval_id _i);
+      LOCAL  (`(eq ctx) (eval_id _ctx);
+      `(eq (Vint (Int.repr (Z.succ (Z.of_nat i) - 1)))) (eval_id _i);
       `(eq (offset_val (Int.repr (Z.succ (Z.of_nat i) * 4)) data)) (eval_id _data);
       `(eq (map Vint (rnd_64 regs K (firstn (S i) bl))))
         (`cons (eval_id _a)
@@ -219,6 +225,7 @@ name i_ _i.
 name T1 _T1.
 name T2 _T2.
 name data_ _data.
+name ctx_ _ctx.
 assert (exists w, nth_error bl i = Some w).
  apply assert_lemmas.nth_error_in_bounds.
 change LBLOCK with 16 in H; omega.
@@ -240,7 +247,6 @@ match goal with
                abbreviate D : tycontext as Delta
 end.
 assert (HDelta'': Delta' = Delta) by reflexivity.
-clear HDelta'.
 rewrite (rnd_64_S _ _ _ _ _ H2 H1).
 forget (rnd_64 regs K (firstn i bl)) as regs'.
 apply semax_pre with
@@ -248,7 +254,8 @@ apply semax_pre with
               exists e, exists f, exists g, exists h,
                 regs' = [a,b,c,d,e,f,g,h])
    LOCAL 
-   (`(eq (offset_val (Int.repr (Z.succ (Z.of_nat i) * 4)) data))
+   (`(eq ctx) (eval_id _ctx);
+   `(eq (offset_val (Int.repr (Z.succ (Z.of_nat i) * 4)) data))
       (eval_id _data);
    `(eq (Vint w)) (eval_id _l);
    `(eq (Vint k)) (eval_id _Ki);
@@ -275,7 +282,173 @@ forget (eq (offset_val (Int.repr (Z.succ (Z.of_nat i) * 4)) data)) as eqofs.
 clear Hdata data.
 replace (Z.succ (Z.of_nat i) - 1)%Z with (Z.of_nat i) by (clear; omega).
 rewrite <- HDelta''; unfold Delta'.
-clear Delta' HDelta'' Delta.
+clear HDelta' Delta' HDelta'' Delta.
 subst regs'.
-eapply rearrange_aux2; eassumption. 
+simple apply rearrange_aux2;
+try apply regs; (* get rid of this line when remove the regs' param of the lemma *)
+ assumption. 
+Qed.
+
+
+Definition f_upto {A} (f: Z -> option A) (bound: Z) (i: Z) : option A :=
+ if zlt i bound then f i else None.
+
+Lemma array_at_f_upto_lo:
+  forall t sh contents lo hi, 
+  array_at t sh (f_upto contents lo) lo hi = array_at_ t sh lo hi.
+Proof.
+intros; apply array_at_ext; intros.
+unfold f_upto; if_tac; auto. omega.
+Qed.
+
+Lemma loop1_aux_lemma1:
+forall sh b i N,
+  length b = N ->
+  i < N ->
+ array_at tuint sh
+       (upd (f_upto (ZnthV tuint b) (Z.of_nat i)) (Z.of_nat i)
+          (Some
+             (big_endian_integer
+                (fun z : Z =>
+                 force_option Int.zero
+                   (ZnthV tuchar
+                      (map Int.repr (intlist_to_Zlist (map swap b)))
+                      (z + Z.of_nat i * 4))))))
+        0 (Z.of_nat N) =
+  array_at tuint sh
+               (f_upto (ZnthV tuint b) (Z.of_nat (S i))) 
+              0 (Z.of_nat N).
+Proof.
+intros.
+apply array_at_ext; intros.
+unfold upd.
+if_tac.
+assert (exists w, nth_error b i = Some w).
+subst N.
+clear - H0.
+revert b H0; induction i; destruct b; simpl; intros; auto.
+omega.
+exists r; reflexivity. 
+inv H0.
+apply IHi; auto. clear - H0.
+apply lt_S_n; auto.
+destruct H3 as [w H3].
+rewrite <- nth_big_endian_integer'' with (w:=w); auto.
+unfold f_upto.
+subst.
+rewrite if_true by (rewrite inj_S; omega).
+unfold ZnthV. rewrite if_false by omega. rewrite Nat2Z.id. auto.
+unfold f_upto.
+if_tac. rewrite if_true by (rewrite inj_S; omega); auto.
+rewrite if_false; auto.
+rewrite inj_S; 
+omega.
+Qed.
+
+Lemma read32_reversed_in_bytearray:
+ forall {Espec: OracleKind} Delta (ofs: int) (lo hi: Z) base e sh contents i P Q
+ (VS:  (var_types Delta) ! ___builtin_read32_reversed = None) 
+ (GS: (glob_types Delta) ! ___builtin_read32_reversed =
+    Some (Global_func (snd __builtin_read32_reversed_spec)))
+ (TE: typeof e = tptr tuint)
+ (CLOQ: Forall (closed_wrt_vars (eq i)) Q)
+ (Hcontents: forall i, (lo <= i < hi)%Z -> isSome (contents i)),
+ PROPx P (LOCALx (tc_environ Delta :: Q) (SEP (TT))) |-- PROP ((lo <= Int.unsigned ofs <= hi-4 )%Z)
+         LOCAL (tc_expr Delta e; `(eq (offset_val ofs base)) (eval_expr e))
+         SEP  (TT) ->
+ semax Delta  (PROPx P (LOCALx Q (SEP (`(array_at tuchar sh contents lo hi base)))))
+        (Scall (Some i)
+           (Evar ___builtin_read32_reversed
+              (Tfunction (Tcons (tptr tuint) Tnil) tuint))
+           [e])
+        (normal_ret_assert
+         (PROP () 
+         (LOCALx (`(eq (Vint (big_endian_integer (fun z => force_option Int.zero (contents (z+Int.unsigned ofs)%Z))))) (eval_id i)
+                        :: Q)                 
+         SEP (`(array_at tuchar sh contents lo hi base))))).
+(*Admitted. *)
+Proof.
+intros.
+apply semax_pre with
+ (PROP  ((lo <= Int.unsigned ofs <= hi - 4)%Z)
+        (LOCALx (tc_expr Delta e :: `(eq (offset_val ofs base)) (eval_expr e) :: Q)
+         (SEP(`(array_at tuchar sh contents lo hi base))))).
+rewrite <- (andp_dup (PROPx P _)).
+eapply derives_trans; [ apply andp_derives | ].
+eapply derives_trans; [ | apply H].
+apply andp_derives; auto.
+apply andp_derives; auto.
+go_lowerx.
+apply sepcon_derives; auto.
+apply TT_right.
+instantiate (1:= PROPx nil (LOCALx Q (SEP  (`(array_at tuchar sh contents lo hi base))))).
+go_lowerx. entailer.
+go_lowerx; entailer.
+normalize.
+clear H.
+normalize.
+rewrite (split_array_at (Int.unsigned ofs)) by omega.
+rewrite (split_array_at (Int.unsigned ofs + 4)%Z) with (hi:=hi) by omega.
+normalize.
+match goal with |- semax _ (PROPx _ (LOCALx _ ?A)) _ _ =>
+ replace A  with (SEPx( [
+         `(array_at tuchar sh contents (Int.unsigned ofs)
+             (Int.unsigned ofs + 4) base)] ++
+               [`(array_at tuchar sh contents lo (Int.unsigned ofs) base),
+         `(array_at tuchar sh contents (Int.unsigned ofs + 4) hi base)]))
+ by (simpl app; apply pred_ext; go_lowerx; cancel)
+end.
+eapply semax_frame1; try reflexivity;
+ [ |  apply derives_refl | auto 50 with closed].
+eapply semax_pre_post.
+Focus 3.
+evar (tl: typelist).
+replace (Tcons (tptr tuint) Tnil) with tl.
+unfold tl.
+eapply semax_call_id1'; try eassumption.
+2: reflexivity.
+apply GS.
+2: reflexivity.
+Unfocus.
+instantiate (3:=nil).
+apply andp_left2.
+instantiate (2:=(offset_val ofs base, sh, fun z => force_option Int.zero (contents (z + Int.unsigned ofs)%Z))).
+cbv beta iota.
+instantiate (1:=nil).
+unfold split; simpl @snd.
+go_lowerx.
+entailer.
+apply andp_right; [apply prop_right; repeat split; auto | ].
+hnf. simpl.
+rewrite TE.
+repeat rewrite denote_tc_assert_andp; repeat split; auto.
+rewrite <- H3.
+rewrite TE.
+destruct base; inv Pbase; reflexivity.
+pattern ofs at 4;
+ replace ofs with (Int.repr (sizeof tuchar * Int.unsigned ofs))%Z
+ by (simpl sizeof; rewrite Z.mul_1_l; apply Int.repr_unsigned).
+rewrite <- offset_val_array_at.
+apply derives_refl'.
+apply equal_f. rewrite Z.add_0_r. apply array_at_ext.
+intros. unfold cSome. rewrite Z.sub_add.
+clear - H5 H0 Hcontents.
+specialize (Hcontents i0);
+ destruct (contents i0); [ | elimtype False; apply Hcontents; omega]. reflexivity.
+2: auto with closed.
+intros; apply andp_left2.
+apply normal_ret_assert_derives'.
+go_lowerx.
+entailer.
+apply derives_refl'.
+pattern ofs at 2;
+ replace ofs with (Int.repr (sizeof tuchar * Int.unsigned ofs))%Z
+ by (simpl sizeof; rewrite Z.mul_1_l; apply Int.repr_unsigned).
+rewrite <- offset_val_array_at.
+apply equal_f. rewrite Z.add_0_r. 
+apply array_at_ext; intros.
+unfold cSome. rewrite Z.sub_add.
+clear - H3 H0 Hcontents.
+specialize (Hcontents i0); destruct (contents i0);
+  [reflexivity | contradiction Hcontents; omega].
 Qed.
