floyd/assert_lemmas.v
@@ -894,6 +894,28 @@ Proof. intros.
 Qed.
 Hint Rewrite add_repr : norm.
 
+Lemma mul_repr:
+ forall x y, Int.mul (Int.repr x) (Int.repr y) = Int.repr (x * y).
+Proof.
+intros. unfold Int.mul.
+apply Int.eqm_samerepr.
+repeat rewrite Int.unsigned_repr_eq.
+apply Int.eqm_mult; unfold Int.eqm; apply Int.eqmod_sym;
+apply Int.eqmod_mod; compute; congruence.
+Qed.
+Hint Rewrite mul_repr : norm.
+
+Lemma sub_repr: forall i j,
+  Int.sub (Int.repr i) (Int.repr j) = Int.repr (i-j).
+Proof.
+  intros.
+ unfold Int.sub.
+ apply Int.eqm_samerepr.
+ unfold Int.eqm.
+ apply Int.eqm_sub; apply Int.eqm_sym; apply Int.eqm_unsigned_repr.
+Qed.
+Hint Rewrite sub_repr : norm.
+
 Lemma int_add_assoc1:
   forall z i j, Int.add (Int.add z (Int.repr i)) (Int.repr j) = Int.add z (Int.repr (i+j)).
 Admitted.
