progs/verif_sha_init.v
@@ -1,0 +1,71 @@
+Require Import floyd.proofauto.
+Require Import progs.sha.
+Require Import progs.SHA256.
+Require Import progs.sha_lemmas.
+Require Import progs.spec_sha.
+Local Open Scope logic.
+
+Lemma array_at_emp:
+ forall t sh f (lo hi: Z) c, (lo >= hi)%Z -> array_at t sh f lo hi c = emp.
+Proof.
+intros.
+unfold array_at, rangespec.
+rewrite nat_of_Z_neg by omega.
+simpl. reflexivity.
+Qed.
+
+Lemma array_at_offset_zero:
+  forall t sh f lo hi c,
+   array_at t sh f lo hi c |-- array_at t sh f lo hi (offset_val (Int.repr 0) (force_ptr c)).
+Proof.
+intros.
+destruct (zlt lo hi).
+saturate_local.
+normalize.
+do 2 rewrite array_at_emp by auto.
+auto.
+Qed.
+
+Hint Resolve array_at_offset_zero : cancel.
+
+Lemma body_SHA256_Init: semax_body Vprog Gtot f_SHA256_Init SHA256_Init_spec.
+Proof.
+start_function.
+name c_ _c.
+revert Delta POSTCONDITION; simpl_typed_mapsto; intros.
+normalize.
+
+replace_SEP 0%Z (`(array_at tuint Tsh (ZnthV tuint nil) 0 8 c)).
+entailer.
+
+Ltac one_store :=
+match goal with |- semax _ _ (Ssequence 
+                              (Sassign (Ederef (Ebinop Oadd _ (Econst_int (Int.repr ?i) _) _) _)  _) _) _ =>
+ forward; [ instantiate (1:=force_option Int.zero (ZnthV tuint init_registers i));
+                 instantiate (1:= i);
+                 entailer!; 
+                 try (apply int_eq_e; compute; reflexivity)
+               | rewrite upd_Znth_next by (compute; reflexivity); simpl app
+               ]
+end.
+one_store.
+one_store.
+one_store.
+one_store.
+one_store.
+one_store.
+one_store.
+one_store.
+forward. (* c->Nl=0; *)
+forward. (* c->Nh=0; *)
+forward. (* c->num=0; *)
+forward. (* return; *)
+unfold sha256state_.
+apply exp_right with (init_registers, (Int.zero, (Int.zero, (nil, Int.zero)))).
+simpl_typed_mapsto.
+unfold s256_h, s256_Nh,s256_Nl, s256_num, s256_data, fst,snd.
+entailer!.
+repeat split.
+simpl; change CBLOCK with 64; omega.
+exists 0; simpl; reflexivity.
+Qed.
