progs/verif_sha_update.v
@@ -1,0 +1,541 @@
+Require Import floyd.proofauto.
+Require Import progs.sha.
+Require Import progs.SHA256.
+Require Import progs.sha_lemmas.
+Require Import progs.spec_sha.
+Local Open Scope logic.
+
+
+Lemma liftSEPlift1:
+ forall (R:  mpred) f, 
+     `(SEP (`R)) f = `R.
+Proof. intros. 
+unfold SEPx. 
+ super_unfold_lift.
+extensionality rho.
+simpl. rewrite sepcon_emp.
+auto.
+Qed.
+
+Definition sha_update_inv sh hashed len c d (frag: list int) data r_Nh r_Nl (done: bool) :=
+   (EX blocks:list int,
+   PROP  (len >= length blocks*4 - length frag /\
+              NPeano.divide LBLOCK (length blocks) /\ 
+              intlist_to_Zlist (map swap blocks) = map Int.unsigned frag ++ firstn (length blocks * 4 - length frag) data /\
+             if done then len-(length blocks*4 - length frag) < CBLOCK else True)
+   LOCAL  (`(eq (offset_val (Int.repr 40) c)) (eval_id _p);
+   `(eq c) (eval_id _c); `(eq (offset_val (Int.repr (Z.of_nat (length blocks*4-length frag))) d)) (eval_id _data);
+   `(eq (Vint (Int.repr (Z.of_nat (len- (length blocks*4 - length frag)))))) (eval_id _len))
+   SEP  (`(array_at tuint Tsh (ZnthV tuint K) 0 (Zlength K)) (eval_var _K256 (tarray tuint 64));
+    `(array_at tuint Tsh (ZnthV tuint (process_msg init_registers (hashed ++ blocks))) 0 8 c);
+    `(sha256_length (hilo r_Nh r_Nl + Z.of_nat len) c);
+   `(array_at_ tuchar Tsh 0 64 (offset_val (Int.repr 40) c));
+   `(field_mapsto_ Tsh t_struct_SHA256state_st _num c);
+   `(data_block sh data d))).
+
+Lemma Hblocks'lem:
+ forall {blocks frag: list int} {data},
+ intlist_to_Zlist (map swap blocks) = map Int.unsigned frag ++ firstn (length blocks * 4 - length frag) data ->
+ length frag <= length blocks * 4.
+Proof.
+intros.
+assert (length (intlist_to_Zlist (map swap blocks)) = 
+               length (   map Int.unsigned frag ++
+     firstn (length blocks * 4 - length frag) data)) by congruence.
+ rewrite length_intlist_to_Zlist, map_length, app_length in H0.
+ rewrite map_length in H0.
+ rewrite mult_comm; omega.
+Qed.
+
+Lemma Hblocks''lem:
+ forall {blocks frag: list int} {data},
+ intlist_to_Zlist blocks = map Int.unsigned frag ++ firstn (length blocks * 4 - length frag) data ->
+ length frag <= length blocks * 4.
+Proof.
+intros.
+assert (length (intlist_to_Zlist blocks) = 
+               length (   map Int.unsigned frag ++
+     firstn (length blocks * 4 - length frag) data)) by congruence.
+ rewrite length_intlist_to_Zlist, app_length, map_length in H0.
+ rewrite mult_comm; omega.
+Qed.
+
+Lemma intro_update_inv:
+ forall (len: nat) (blocks : list int) (frag: list int) (data: list Z) (P' Q: Prop),
+  (forall (Hblocks_len: len >= length blocks * 4 - length frag)
+            (Hdiv: NPeano.divide LBLOCK (length blocks))
+            (Hblocks: intlist_to_Zlist (map swap blocks) = map Int.unsigned frag ++ firstn (length blocks * 4 - length frag) data)
+            (DONE: P')
+            (Hblocks': length blocks * 4 >= length frag),
+            Q) ->
+    (len >= length blocks*4 - length frag /\
+    NPeano.divide LBLOCK (length blocks) /\ 
+    intlist_to_Zlist (map swap blocks) = map Int.unsigned frag ++ firstn (length blocks * 4 - length frag) data /\
+              P' -> Q). 
+Proof.
+intros.
+ destruct H0 as  [Hblocks_len [Hdiv [Hblocks DONE]]].
+ apply H; clear H; auto.
+ apply Hblocks'lem in Hblocks; auto.
+Qed.
+
+Lemma split3_data_block:
+  forall lo n sh data d,
+  lo+n <= length data ->
+  data_block sh data d = 
+  data_block sh (firstn lo data) d *
+  data_block sh (firstn n (list_drop lo data)) (offset_val (Int.repr (Z.of_nat lo)) d) *
+  data_block sh (list_drop (lo+n) data)  (offset_val (Int.repr (Z.of_nat (lo+n))) d).
+Admitted.
+
+ Lemma divide_length_app:
+ forall {A} n (al bl: list A), 
+      NPeano.divide n (length al) -> 
+      NPeano.divide n (length bl) ->
+      NPeano.divide n (length (al++bl)).
+Proof.
+ intros. destruct H,H0. exists (x+x0).
+ rewrite app_length,H,H0;  rewrite  mult_plus_distr_r; omega.
+Qed.
+
+Lemma SHA256_Update_aux:
+ forall (Espec : OracleKind) (sh: share) (hashed : list int) (r_data: list int) (data : list Z) (c d : val)
+  (len : nat) (r_h : list int) (r_Nl r_Nh : int)
+   (Delta : tycontext) (blocks bl : list int)
+ (HDelta: Delta = initialized _p (initialized _n (initialized _data
+                     (func_tycontext f_SHA256_Update Vprog Gtot))))
+ (H: len <= length data)
+ (Hdiv: NPeano.divide LBLOCK (length blocks))
+ (HBOUND: (s256a_len (S256abs hashed (map Int.unsigned r_data)) < BOUND)%Z)
+ (H0: r_h = process_msg init_registers hashed)
+ (H1: Zlength (intlist_to_Zlist hashed ++ map Int.unsigned r_data) = hilo r_Nh r_Nl)
+ (H4: NPeano.divide LBLOCK (length hashed))
+ (Hblocks: intlist_to_Zlist (map swap blocks) = (map Int.unsigned r_data) ++ firstn (length blocks * 4 - length r_data) data)
+ (H3 : length (map Int.unsigned r_data) < CBLOCK)
+ (Hlen: (Z.of_nat len <= Int.max_unsigned)%Z)
+ (Hlen_ge: len - (length blocks * 4 - length r_data) >= CBLOCK)
+ (H6: firstn CBLOCK (list_drop (length blocks * 4 - length r_data) data) =
+     intlist_to_Zlist (map swap bl))
+ (H7: length bl = LBLOCK),
+semax Delta
+  (PROP  ()
+   LOCAL 
+   (`(typed_true
+        (typeof
+           (Ebinop Oge (Etempvar _len tuint)
+              (Ebinop Omul (Econst_int (Int.repr 16) tint)
+                 (Econst_int (Int.repr 4) tint) tint) tint)))
+      (eval_expr
+         (Ebinop Oge (Etempvar _len tuint)
+            (Ebinop Omul (Econst_int (Int.repr 16) tint)
+               (Econst_int (Int.repr 4) tint) tint) tint));
+   `(eq (offset_val (Int.repr 40) c)) (eval_id _p); `(eq c) (eval_id _c);
+   `(eq
+       (offset_val (Int.repr (Z.of_nat (length blocks * 4 - length r_data)))
+          d)) (eval_id _data);
+   `(eq
+       (Vint
+          (Int.repr (Z.of_nat (len - (length blocks * 4 - length r_data))))))
+     (eval_id _len))
+   SEP 
+   (`(array_at tuint Tsh (ZnthV tuint K) 0 (Zlength K)) (eval_var _K256 (tarray tuint 64));
+    `(array_at tuint Tsh
+        (ZnthV tuint (process_msg init_registers (hashed ++ blocks))) 0 8 c);
+   `(sha256_length (hilo r_Nh r_Nl + Z.of_nat len) c);
+   `(array_at_ tuchar Tsh 0 64 (offset_val (Int.repr 40) c));
+   `(field_mapsto_ Tsh t_struct_SHA256state_st _num c);
+   `(data_block sh data d)))
+  (Ssequence
+     (Scall None
+        (Evar _sha256_block_data_order
+           (Tfunction
+              (Tcons (tptr t_struct_SHA256state_st) (Tcons (tptr tvoid) Tnil))
+              tvoid))
+        [Etempvar _c (tptr t_struct_SHA256state_st),
+        Etempvar _data (tptr tuchar)])
+     (Ssequence
+        (Sset _data
+           (Ebinop Oadd (Etempvar _data (tptr tuchar))
+              (Ebinop Omul (Econst_int (Int.repr 16) tint)
+                 (Econst_int (Int.repr 4) tint) tint) (tptr tuchar)))
+        (Sset _len
+           (Ebinop Osub (Etempvar _len tuint)
+              (Ebinop Omul (Econst_int (Int.repr 16) tint)
+                 (Econst_int (Int.repr 4) tint) tint) tuint))))
+  (loop1_ret_assert
+     (sha_update_inv sh hashed len c d r_data data r_Nh r_Nl false)
+     (normal_ret_assert
+        (sha_update_inv sh hashed len c d r_data data r_Nh r_Nl true))).
+Proof.
+intros.
+name c' _c.
+name data_ _data_.
+name len' _len.
+name data' _data.
+name p _p.
+name n _n.
+subst Delta; simplify_Delta; abbreviate_semax.
+forward. (* sha256_block_data_order (c,data); *)
+instantiate (1:=(hashed++ blocks, 
+                           bl,
+                           c, 
+                           offset_val (Int.repr (Z.of_nat (length blocks * 4 - length r_data))) d,
+                           sh)) in (Value of witness).
+ instantiate (1:= [
+   `(sha256_length (hilo r_Nh r_Nl + Z.of_nat len) c),
+  `(array_at_ tuchar Tsh 0 64 (offset_val (Int.repr 40) c)),
+  `(field_mapsto_ Tsh t_struct_SHA256state_st _num c),
+  `(data_block sh (firstn (length blocks * 4 - length r_data)  data) d),
+  `(data_block sh (list_drop (length blocks * 4 - length r_data + CBLOCK) data) 
+                 (offset_val (Int.repr (Z.of_nat (length blocks * 4 - length r_data + CBLOCK))) d))])
+    in (Value of Frame).
+ unfold Frame, witness; clear Frame witness.
+ cbv beta iota.
+entailer!.
+rewrite mul_repr in H5; rewrite H5; reflexivity.
+apply divide_length_app; auto.
+ replace (eval_var _K256 (tarray tuint 64)
+         (env_set
+            (env_set (globals_only rho) _in
+               (offset_val
+                  (Int.repr (Z.of_nat (length blocks * 4 - length r_data))) d))
+            _ctx c')) with (eval_var _K256 (tarray tuint 64) rho)
+ by (repeat rewrite eval_var_env_set; 
+      erewrite elim_globals_only by (split3; [eassumption | reflexivity.. ]);
+       reflexivity).
+ rewrite <- H6.
+ rewrite (split3_data_block (length blocks * 4 - length r_data) CBLOCK sh data) by omega.
+ cancel.
+
+replace_SEP 0%Z
+  (`(array_at tuint Tsh
+          (ZnthV tuint
+             (process_msg init_registers ((hashed ++ blocks) ++ bl))) 0 8 c) *
+      `(data_block sh (intlist_to_Zlist (map swap bl))
+          (offset_val
+             (Int.repr (Z.of_nat (length blocks * 4 - length r_data))) d)) *
+      `(array_at tuint Tsh (ZnthV tuint K) 0 (Zlength K))
+        (eval_var _K256 (tarray tuint 64))).
+ entailer!.
+  erewrite elim_globals_only by (split3; [eassumption | reflexivity.. ]);
+  auto.
+ normalize.
+
+ forward. (* data += SHA_CBLOCK; *)
+ entailer. 
+ forward. (* len  -= SHA_CBLOCK; *)
+ unfold loop1_ret_assert.
+ unfold sha_update_inv.
+ apply exp_right with (blocks++ bl).
+ entailer.
+ clear TC0 TC.
+ rewrite negb_true_iff in H8.
+ unfold Int.ltu in H8.
+ if_tac in H8; inv H8.
+ rewrite mul_repr in H0.
+ change (Int.unsigned (Int.repr (16 * 4)))%Z with 64%Z in H0.
+ rewrite Int.unsigned_repr in H0
+  by (clear - Hlen; split; [omega | ];
+        rewrite Nat2Z.inj_sub_max;
+        apply Z.max_lub; omega).
+
+ assert (Hblocks' := Hblocks'lem Hblocks).
+ apply andp_right; [ apply prop_right; repeat split | cancel].
+*
+ rewrite app_length.
+ rewrite  mult_plus_distr_r. 
+ rewrite plus_comm.
+ rewrite <- NPeano.Nat.add_sub_assoc by (clear - Hblocks'; omega).
+ rewrite H7.
+ clear - H0.
+ rewrite Nat2Z.inj_sub_max in H0.
+ rewrite Zmax_spec in H0. if_tac in H0; try omega.
+ clear H.
+ apply Nat2Z.inj_ge.
+ rewrite Nat2Z.inj_add.
+ change (Z.of_nat (LBLOCK*4)) with 64%Z. omega.
+* rewrite app_length.
+ clear - Hdiv H7. rewrite H7. destruct Hdiv as [x ?]; exists (S x).
+ simpl; omega.
+*
+ rewrite map_app; rewrite intlist_to_Zlist_app.
+ rewrite Hblocks; rewrite <- H6.
+ rewrite app_ass.
+ f_equal. rewrite app_length. rewrite H7.
+  rewrite  mult_plus_distr_r. change (LBLOCK*4)%nat with CBLOCK.
+ rewrite NPeano.Nat.add_sub_swap by auto.
+ apply firstn_app.
+*
+ destruct d; inv Pd; simpl. f_equal.
+ rewrite Int.add_assoc. f_equal.
+ rewrite mul_repr.
+ rewrite app_length.
+ rewrite H7.
+ rewrite add_repr.
+ f_equal.
+ rewrite  mult_plus_distr_r.
+ change (LBLOCK*4) with CBLOCK.
+rewrite NPeano.Nat.add_sub_swap by auto.
+ rewrite Nat2Z.inj_add.
+ f_equal.
+*
+ f_equal.
+ rewrite app_length. rewrite mult_plus_distr_r. rewrite H7.
+ change (16*4)%Z with  (Z.of_nat (LBLOCK*4)).
+ symmetry.  rewrite <- Nat2Z.inj_sub by auto.
+ f_equal.
+ rewrite <- NPeano.Nat.sub_add_distr by auto.
+ f_equal.
+ rewrite NPeano.Nat.add_sub_swap by auto.
+ auto.
+*
+ rewrite app_ass.
+ rewrite (split3_data_block (length blocks * 4 - length r_data) CBLOCK sh data)
+  by omega.
+ cancel.
+apply derives_refl'. f_equal. auto.
+Qed.
+
+Lemma elim_globals_only': 
+ forall a: mpred, 
+ (@liftx (Tarrow environ (LiftEnviron mpred)) (`a) globals_only) = `a.
+Proof. reflexivity. Qed.
+
+Lemma Zlength_intlist_to_Zlist_app:
+ forall al bl,  Zlength (intlist_to_Zlist (al++bl)) =
+    (Zlength (intlist_to_Zlist al) + Zlength (intlist_to_Zlist bl))%Z.
+Proof.
+Admitted.
+
+Lemma body_SHA256_Update: semax_body Vprog Gtot f_SHA256_Update SHA256_Update_spec.
+Proof.
+start_function.
+name c' _c.
+name data_ _data_.
+name len' _len.
+name data' _data.
+name p _p.
+name n _n.
+name fragment _fragment.
+rename H0 into HBOUND.
+forward.  (* data=data_; *)
+
+unfold sha256_length, sha256state_.
+normalize.
+intros [r_h [r_Nl [r_Nh [r_data r_num]]]].
+normalize.
+unfold s256a_len.
+unfold s256_relate in H0.
+destruct a as [hashed data0].
+simpl_typed_mapsto.
+unfold s256_h, s256_Nh,s256_Nl, s256_num, s256_data, fst,snd in H0|-*.
+destruct H0 as [? [? [? [? [? ?]]]]].
+revert POSTCONDITION; subst data0.
+intro.
+subst r_h.
+
+forward.  (* SHA256_addlength(c, len); *)
+instantiate (1:= (len,c, hilo r_Nh r_Nl)) in (Value of witness).
+entailer!.
+unfold sha256_length.
+normalize; apply exp_right with r_Nl. 
+normalize; apply exp_right with r_Nh.
+entailer!.
+cbv beta iota.
+normalize.
+rewrite elim_globals_only'.
+
+forward. (* n = c->num; *)
+forward. (* p=c->data; *)
+entailer. simpl.
+apply semax_pre with
+ (PROP  ( (Z.of_nat len <= Int.max_unsigned)%Z)
+   LOCAL 
+   (`(eq  (offset_val (Int.repr 40) c)) (eval_id _p);
+   `(eq (Vint r_num)) (eval_id _n);
+   `(eq c) (eval_id _c); `(eq d) (eval_id _data);
+   `(eq (Vint (Int.repr (Z.of_nat len)))) (eval_id _len))
+   SEP  (`(array_at tuint Tsh (ZnthV tuint (process_msg init_registers hashed)) 0 8 c);
+    `(sha256_length (hilo r_Nh r_Nl + Z.of_nat len) c);
+   `(array_at tuchar Tsh (ZnthV tuchar r_data) 0 64 (offset_val (Int.repr 40) c));
+   `(field_mapsto Tsh t_struct_SHA256state_st _num c (Vint r_num));
+   `(array_at tuint Tsh (ZnthV tuint K) 0 (Zlength K))  (eval_var _K256 (tarray tuint 64));
+   `(data_block sh data d))).
+entailer!.
+rewrite H2.
+destruct (Int.unsigned_range_2 len'); auto.
+rewrite H2; apply Int.repr_unsigned.
+apply semax_extract_PROP; intro Hlen.
+
+forward_if (sha_update_inv sh hashed len c d r_data data r_Nh r_Nl false).
+* entailer!.   (* cond-expression typechecks *)
+* (* then clause *)
+forward.  (* fragment = SHA_CBLOCK-n; *)
+rewrite semax_seq_skip.
+forward_if (sha_update_inv sh hashed len c d r_data data r_Nh r_Nl false).
+ + entailer!.  (* cond-expression typechecks *)
+    rewrite H2; reflexivity.
+ + (* then clause: len >= fragment *)
+    admit.
+ + (* else clause: len < fragment *)
+    admit.
+ + forward. (* bogus skip *)
+    rewrite overridePost_normal'.
+    apply andp_left2; auto.
+* (* else clause *)
+forward.  (* skip; *)
+rewrite overridePost_normal'.
+apply exp_right with nil. rewrite <- app_nil_end.
+entailer.
+ rewrite negb_false_iff in H2;  apply int_eq_e in H2; subst n;
+ destruct r_data; inv H5.
+ apply andp_right; [apply prop_right; repeat split | ].
+ + clear; omega.
+ + exists 0; reflexivity.
+ +  repeat f_equal; omega.
+ + rewrite <- app_nil_end. cancel.
+* (* after if (n!=0) *)
+eapply semax_seq' with
+     (sha_update_inv sh hashed len c d r_data data r_Nh r_Nl true).
+apply semax_while.
++ reflexivity.
++ entailer!.
++ rewrite normal_ret_assert_elim.
+  unfold sha_update_inv.
+  normalize.
+  rewrite andp_assoc; do 2 rewrite insert_local.
+  apply exp_right with blocks.
+  entailer.
+  rename H7 into Hblocks;  assert (Hblocks' := Hblocks'lem Hblocks).
+  apply prop_right.
+  change (Int.mul (Int.repr 16) (Int.repr 4)) with (Int.repr 64) in H8;
+  rewrite negb_false_iff in H8;
+  apply Int.ltu_inv in H8.  
+  rewrite Int.unsigned_repr in H8.
+  destruct H8 as [_ H8].
+  apply Nat2Z.inj_lt.
+ apply H8.
+  split; [ clear; omega | ].
+  rewrite Nat2Z.inj_sub by auto. omega.
++ unfold LOOP_BODY, abbreviate; clear LOOP_BODY MORE_COMMANDS POSTCONDITION.
+  unfold sha_update_inv at 1.
+  normalize.
+  apply extract_exists_pre; intro blocks.
+  rewrite insert_local.
+  apply semax_extract_PROP; apply intro_update_inv; intros.
+ match goal with |- semax _ (PROPx _ ?QR) _ _ =>
+ apply semax_pre with (PROP (len - (length blocks*4 - length r_data) >= CBLOCK) QR)
+ end.
+ {entailer.
+  rewrite mul_repr in H2; rewrite H2. 
+  apply prop_right; split; [ | reflexivity].
+  rewrite negb_true_iff in H2;
+   unfold Int.ltu in H2;
+  if_tac in H2; inv H2.
+  rewrite Int.unsigned_repr in H6;
+  change (Int.unsigned (Int.mul (Int.repr 16) (Int.repr 4)))
+    with (Z.of_nat CBLOCK) in H6.
+  apply Nat2Z.inj_ge.
+ apply H6.
+  split; [clear; omega | ].
+  rewrite Nat2Z.inj_sub by auto.
+  omega.
+}
+
+Lemma exists_intlist_to_Zlist':
+  forall n (al: list Z), 
+   length al = (n * 4)%nat ->
+   exists bl, al = intlist_to_Zlist (map swap bl) /\ length bl = n.
+Admitted.
+
+  apply semax_extract_PROP; intro Hlen_ge.
+  destruct (exists_intlist_to_Zlist' LBLOCK (firstn CBLOCK (list_drop (length blocks*4 - length r_data) data)))
+      as [bl [? ?]].
+  rewrite firstn_length.
+  rewrite min_l; [reflexivity |].
+ rewrite list_drop_length.
+  transitivity (len - (length blocks*4 - length r_data)); [ | clear - H; omega].
+  apply Hlen_ge.
+  clear - Hlen_ge H H3 H5 ; omega.
+ simple apply (SHA256_Update_aux Espec sh hashed r_data data c d len (process_msg init_registers hashed) r_Nl r_Nh Delta blocks bl); 
+   try assumption.
+simplify_Delta; reflexivity.
+reflexivity.
++
+  abbreviate_semax.
+  unfold sha_update_inv.   apply extract_exists_pre; intro blocks.
+  apply semax_extract_PROP; apply intro_update_inv; intros.
+  forward.    (* c->num=len; *)
+  forward_if  (EX  a' : s256abs,
+                    PROP  (update_abs (firstn len data) (S256abs hashed (map Int.unsigned r_data)) a')
+                    LOCAL ()
+                    SEP 
+                    (`(array_at tuint Tsh (ZnthV tuint K) 0 (Zlength K))
+                       (eval_var _K256 (tarray tuint 64));
+                    `(sha256state_ a' c); `(data_block sh data d))).
+ entailer.
+ admit.  (* then-clause *)
+ forward. (* else-clause *)
+ normalize.
+ rewrite overridePost_normal'.
+ apply exp_right 
+   with (S256abs (hashed++blocks) nil).
+ entailer.
+ rewrite negb_false_iff in H2; apply int_eq_e in H2.
+ assert (H2': Int.unsigned (Int.repr (Z.of_nat (len - (length blocks * 4 - length r_data)))) = 
+              Int.unsigned Int.zero) by (f_equal; apply H2).
+ rewrite Int.unsigned_zero in H2'.
+ rewrite Int.unsigned_repr in H2'
+ by (split; [clear; omega | rewrite Nat2Z.inj_sub by auto; clear - Hlen; omega]).
+ assert (H7: len = length blocks * 4 - length r_data).
+   rewrite Nat2Z.inj_sub in H2' by auto.
+    apply Nat2Z.inj. clear - H2'; omega.
+ apply andp_right.
+ apply prop_right.
+ constructor; auto.
+ change CBLOCK with 64; simpl; clear; omega.
+ rewrite <- app_nil_end.
+ rewrite Hblocks.
+ rewrite <- H7.
+ reflexivity.
+ unfold sha256state_.
+ cancel.
+ unfold sha256_length.
+ normalize.
+ apply exp_right with 
+              (process_msg init_registers (hashed ++ blocks),
+                (lo, (hi, (nil, 
+                 Int.zero)))).
+ simpl_typed_mapsto; unfold s256_relate.
+unfold s256_h, s256_Nh,s256_Nl, s256_num, s256_data, fst,snd.
+ apply andp_right; [apply prop_right | cancel].
+ repeat split; simpl; auto.
+ rewrite <- app_nil_end.
+ rewrite Zlength_intlist_to_Zlist_app.
+ replace (Zlength (intlist_to_Zlist blocks)) with
+    (Zlength (intlist_to_Zlist (map swap blocks)))
+ by (repeat rewrite Zlength_correct, length_intlist_to_Zlist; rewrite map_length; reflexivity).
+ rewrite Hblocks.
+ rewrite H6.
+ rewrite H7.
+ rewrite Nat2Z.inj_sub by auto.
+ rewrite (Zlength_correct (_ ++ _)).
+ rewrite app_length. rewrite map_length. rewrite Nat2Z.inj_add.
+ rewrite <- H1.
+ repeat rewrite Zlength_correct; rewrite app_length; rewrite map_length.
+ rewrite firstn_length.
+ rewrite min_l.  rewrite Nat2Z.inj_add.
+ rewrite Nat2Z.inj_sub by auto.
+ clear; omega.
+ omega.
+ change CBLOCK with 64; clear; omega.
+ apply divide_length_app; auto.
+ rewrite H2'.
+ cancel.
+ apply extract_exists_pre; intro a'.
+ forward.
+ apply exp_right with a'.
+ entailer.
+ erewrite elim_globals_only by (split3; [eassumption | reflexivity.. ]).
+ cancel.
+Qed.
